`compile`: Complete defs & prove semantics preservation

SoftwareFoundations2/StackMachine/Compile.lean
@@ -6,23 +6,26 @@ def AExp.compile : AExp → List Instruction
   | ANum n       => [ PUSH n ]
   | AId x        => [ LOAD x ]
   | AMult a1 a2  => a1.compile ++ a2.compile ++ [ MUL ]
-  | AMinus a1 a2 => sorry
-  | APlus a1 a2  => sorry
+  | AMinus a1 a2 => a1.compile ++ a2.compile ++ [ SUB ]
+  | APlus a1 a2  => a1.compile ++ a2.compile ++ [ ADD ]
 
 def BExp.compile : BExp → List Instruction
   | BTrue        => [ PUSH 1 ]
   | BFalse       => [ PUSH 0 ]
   | BEq a1 a2    => a1.compile ++ a2.compile ++ [ EQ ]
-  | BNeq a1 a2   => sorry
+  | BNeq a1 a2   => a1.compile ++ a2.compile ++ [ EQ, ISZERO ]
   | BLe a1 a2    => a1.compile ++ a2.compile ++ [ .LE ]
-  | BGt a1 a2    => sorry
-  | BNot b       => sorry
-  | BAnd b1 b2   => sorry
+  | BGt a1 a2    => a1.compile ++ a2.compile ++ [ .LE, ISZERO ]
+  | BNot b       => b.compile ++ [ISZERO]
+  | BAnd b1 b2   => b1.compile ++ b2.compile ++ [ MUL ]
 
 def Com.compileOffset (pcOffset : ℕ) : Com → List Instruction
-  | CSkip       => sorry
-  | CAsgn x a   => sorry
-  | CSeq c1 c2  => sorry
+  | CSkip       => [ NOP ]
+  | CAsgn x a   => a.compile ++ [ STORE x ]
+  | CSeq c1 c2  =>
+      let c1c := c1.compileOffset pcOffset
+      let c2c := c2.compileOffset (pcOffset + c1c.length)
+      c1c ++ c2c
   | CIf b c1 c2 =>
       -- See comment below for stack layout
       let bCode := b.compile
@@ -47,7 +50,7 @@ def Com.compileOffset (pcOffset : ℕ) : Com → List Instruction
 def Com.compile (com : Com) := com.compileOffset 0 ++ [.STOP]
 
 /-
-  Stack layout for a compiled `if b then l1 else l2`.
+  Code layout for a compiled `if b then l1 else l2`.
   First column: code section;
   Second column: offset within the code.
 
@@ -64,21 +67,18 @@ def Com.compile (com : Com) := com.compileOffset 0 ++ [.STOP]
       JUMP             pcOffset + bCode.length + l1.length + l2.length + 7
                        pcOffset + bCode.length + l1.length + l2.length + 8   { == pcJumpPost }
 
-  Stack layout for a compiled `while b do l od`:
+  Code layout for a compiled `while b do l od`:
 
       bCode            pcOffset                                              { == pcCheck }
       pcJumpTrue       pcOffset + bCode.length
       JUMPI            pcOffset + bCode.length + 1
-      pcJumpPost       pcOffset + bCode.length + 2      
+      pcJumpPost       pcOffset + bCode.length + 2
       JUMP             pcOffset + bCode.length + 3
       l                pcOffset + bCode.length + 4                           { == pcJumpTrue }
       pcCheck          pcOffset + bCode.length + l.length + 4
       JUMP             pcOffset + bCode.length + l.length + 5
                        pcOffset + bCode.length + l.length + 6                { == pcJumpPost }
 -/
-
-/-
-  Uncomment after filling all sorries:
 
 #eval aexp⟨{ (x * 2) - 1 + 30 }⟩.compile
 #eval aexp⟨{ x - (2 * y) }⟩.compile
@@ -136,4 +136,3 @@ def Com.compile (com : Com) := com.compileOffset 0 ++ [.STOP]
   pc    := 0,
   mem   := [ "x" ↦ 161 ],
 })
--/
