SoftwareFoundations2/StackMachine/Semantics.lean
@@ -44,9 +44,11 @@ def step (μ : MachineState) : ExecutionState := do
       let ⟨n1, n2, s⟩ ← stackPeek2 μ
       .ok <| replaceStackAndIncrPC μ ((n2 + n1) :: s)
   | SUB      =>
-      sorry
+      let ⟨n1, n2, s⟩ ← stackPeek2 μ
+      .ok <| replaceStackAndIncrPC μ ((n2 - n1) :: s)
   | MUL      =>
-      sorry
+      let ⟨n1, n2, s⟩ ← stackPeek2 μ
+      .ok <| replaceStackAndIncrPC μ ((n2 * n1) :: s)
   | EQ       =>
       let ⟨n1, n2, s⟩ ← stackPeek2 μ
       if n2 == n1 then
@@ -54,9 +56,17 @@ def step (μ : MachineState) : ExecutionState := do
       else
         .ok <| replaceStackAndIncrPC μ (0 :: s)
   | .LE       =>
-      sorry
+      let ⟨n1, n2, s⟩ ← stackPeek2 μ
+      if n2 ≤ n1 then
+        .ok <| replaceStackAndIncrPC μ (1 :: s)
+      else
+        .ok <| replaceStackAndIncrPC μ (0 :: s)
   | .ISZERO     =>
-      sorry
+      let ⟨n1, s⟩ ← stackPeek1 μ
+      if n1 == 0 then
+        .ok <| replaceStackAndIncrPC μ (1 :: s)
+      else
+        .ok <| replaceStackAndIncrPC μ (0 :: s)
   | JUMP =>
       let ⟨pc, s⟩ ← stackPeek1 μ
       .ok <| { μ with pc := pc, stack := s }
