SoftwareFoundations2/StackMachine/Lemmas.lean
@@ -15,42 +15,122 @@ attribute [local simp] fetchInstr
 attribute [local simp] stackPeek2
 attribute [local simp] stackPeek1
 
-set_option warn.sorry false in
 lemma isErrorLemma {err st'} : ¬ Reachable (.error err) st' := by
-  sorry
+  intros h
+  generalize eq : (Except.error err) = st at h
+  induction h with
+  | step h => cases eq
+  | trans s1 s2 ih1 ih2 =>
+    cases eq
+    simp only [imp_false, not_true_eq_false] at ih1
 
-set_option warn.sorry false in
 lemma isOOFLemma {st} : ¬ Reachable st (.error .OutOfFuel) := by
-  sorry
+  intros h
+  generalize eq : (Except.error ExecutionException.OutOfFuel) = st' at h
+  induction h with
+  | @step μ _ h =>
+    cases eq
+    simp [step, Bind.bind, Except.bind] at h
+    aesop
+  | trans s1 s2 ih1 ih2 =>
+    cases eq
+    simp only [imp_false, not_true_eq_false] at ih2
 
-set_option warn.sorry false in
 lemma isFinalStepLemma {μ st} (h : isFinal (.ok μ)) :
     step μ = st → isError st := by
-  sorry
+  rw [isFinal] at h
+  simp only [step, bind, Except.bind, fetchInstr, h, Nat.lt_irrefl, ↓reduceDIte]
+  intro h1
+  rw [←h1, isError]
+  trivial
 
-set_option warn.sorry false in
 lemma isFinalLemma {st st'} (h : isFinal st) :
     Reachable st st' → isError st' := by
-  sorry
+  intro h
+  induction h with
+  | @step μ st'' hx =>
+    exact isFinalStepLemma h hx
+  | @trans _ stx st'' s1 s2 ih1 ih2 =>
+    apply ih1 at h
+    cases st'' with
+    | ok => contradiction
+    | error e =>
+      have := @isErrorLemma e stx
+      contradiction
 
-set_option warn.sorry false in
 lemma executeFinal {μ st fuel} (h : isFinal (.ok μ)) :
     execute fuel μ = st → st = .ok μ := by
-  sorry
+  intro h1
+  rw [execute.eq_def] at h1
+  simp [h] at h1
+  symm
+  assumption
 
-set_option warn.sorry false in
 lemma executeExtend {μ μ' fuel} (h : step μ = .ok μ') :
     execute (fuel + 1) μ = execute fuel μ' := by
-  sorry
+  rw [execute]
+  by_cases hx : μ.pc < μ.code.length
+  · rw [h]
+    by_cases hf : isFinal (Except.ok μ)
+    · rw [isFinal] at hf
+      aesop
+    · simp [hf]
+  · simp [step, hx, Bind.bind, Except.bind] at h
 
-set_option warn.sorry false in
 lemma executeStepFinal {μ st} (h1 : isFinal st) (h2 : step μ = st) :
     execute 1 μ = st := by
-  sorry
+    rw [execute]
+    by_cases hx : μ.pc < μ.code.length
+    · have hf : ¬ isFinal (Except.ok μ) := by
+        rw [isFinal]
+        intro habs
+        rw [habs] at hx
+        exact Nat.lt_irrefl μ.code.length hx
+      rw [h2]
+      simp only [hf, ↓reduceIte]
+      cases st with
+      | ok μ' =>
+        simp only [execute, ite_eq_left_iff, reduceCtorEq, imp_false, Decidable.not_not]
+        exact h1
+      | error => contradiction
+    · simp only [step, bind, Except.bind, fetchInstr, hx, ↓reduceDIte] at h2
+      rw [←h2] at h1
+      contradiction
 
-set_option warn.sorry false in
+lemma executeLemmaAux {n : Nat} {μ μ' : MachineState} (h : Reachable (.ok μ) (.ok μ'))
+  : ∃m, execute m μ = execute n μ' := by
+  generalize eq1 : Except.ok μ = st at h
+  generalize eq2 : Except.ok μ' = st' at h
+  induction h generalizing n μ μ' with
+  | step hs =>
+    cases eq1
+    cases eq2
+    use n + 1
+    exact executeExtend hs
+  | @trans _ _ sti _ _ ih1 ih2 =>
+    cases eq1
+    cases eq2
+    simp only [Except.ok.injEq, forall_eq_apply_imp_iff] at *
+    cases sti with
+    | error x =>
+      have := @isErrorLemma x (Except.ok μ')
+      contradiction
+    | ok μi =>
+      specialize @ih2 n μi rfl
+      obtain ⟨m2, hm2⟩ := ih2
+      specialize @ih1 m2 μ μi rfl rfl
+      obtain ⟨m1, hm1⟩ := ih1
+      rw [hm2] at hm1
+      use m1
+
 /-- Hard exercise, you will likely need the lemmas above,
     and possibly additional intermediary results. -/
 lemma executeLemma {μ st} (h1 : Reachable (.ok μ) st) (h2 : isFinal st) :
     ∃ fuel : ℕ, execute fuel μ = st := by
-  sorry
+  cases st with
+  | error => contradiction
+  | ok μx =>
+    obtain ⟨m, hm⟩ := @executeLemmaAux 0 _ _ h1
+    use m
+    rw [hm, execute]
+    simp [h2]
